Fine/Completeness/SystemB.lean
@@ -2,8 +2,12 @@ import Fine.Semantics.Model
 import Fine.Semantics.Satisfaction
 import Fine.Hilbert.SystemB
 import Fine.PropositionalLanguage
+import Mathlib.Data.Finset.Basic
+import Mathlib.Init.Set
 
 def formalTheory (Γ : Ctx) : Prop := ∀f : Form, f ∈ Γ ↔ Γ ⊢ f
+
+abbrev Th := { Γ : Ctx // formalTheory Γ }
 
 def generatedTheory (Γ : Ctx) : Ctx := BProvable Γ
 
@@ -33,6 +37,8 @@ theorem generatedFormal : ∀Γ : Ctx, formalTheory (▲Γ) := by
 def DisjunctionClosed (Γ : Ctx) := ∀f g : Form, f ∈ Γ ∧ g ∈ Γ → f ¦ g ∈ Γ
 
 def PrimeTheory (Γ : Ctx) := ∀f g : Form, f ¦ g ∈ Γ → f ∈ Γ ∨ g ∈ Γ
+
+abbrev Pr := { Γ : Th // PrimeTheory Γ }
 
 def FormalApplication (Γ : Ctx) (Δ : Ctx) : Ctx := 
   λf : Form => ∃g : Form, g ∈ Δ ∧ (g ⊃ f) ∈ Γ
@@ -79,3 +85,29 @@ lemma BisFormal : formalTheory BTheory := by
       have ⟨l₁,_⟩ := ih₁ ⟨prf₁,trivial⟩
       have ⟨l₂,_⟩ := ih₂ ⟨prf₂,trivial⟩
       exact ⟨BTheorem.adj l₁ l₂, trivial⟩
+
+theorem BProof.compactness { Γ : Ctx } { f : Form } : BProof Γ f → Σs : Finset Form, BProof ↑s f := by
+  intros prf₁; induction prf₁
+  case ax g _ => 
+    have l₁ : g ∈ {g} := Finset.mem_singleton.mpr rfl
+    have l₂ : ({g} : Finset Form) = ({g} : Ctx) := Finset.coe_singleton g
+    have prf₂ : BProof ↑{g} g := by
+      rw [←l₂]
+      apply ax l₁
+    rw [←l₂] at prf₂
+    exact ⟨↑{g}, prf₂⟩
+  case mp P Q _ h₂ ih => 
+    have ⟨fin, prf⟩ := ih
+    exact ⟨fin, mp prf h₂⟩
+  case adj P Q _ _ ih₁ ih₂ => 
+    have ⟨fin₁, prf₁⟩ := ih₁
+    have ⟨fin₂, prf₂⟩ := ih₂
+    have prf₃ : BProof (↑fin₁ ∪ ↑fin₂) P := BProof.monotone (Set.subset_union_left ↑fin₁ ↑fin₂) prf₁
+    have prf₄ : BProof (↑fin₁ ∪ ↑fin₂) Q := BProof.monotone (Set.subset_union_right ↑fin₁ ↑fin₂) prf₂
+    have prf₅ := adj prf₃ prf₄
+    rw [←Finset.coe_union] at prf₅
+    exact ⟨↑(fin₁ ∪ fin₂), prf₅⟩
+
+def formalApplicationFunction : Th → Th → Th := sorry
+
+def formalStarFunction : Pr → Pr := sorry
